add existence part of thm (term alg is free)

src/term.lean
@@ -10,7 +10,7 @@ open lattice
 
 -- The next few structures are direct translations of Andrej Bauer's Coq code
 -- at https://gist.github.com/andrejbauer/3cc438ab38646516e5e9278fdb22022c
-
+--section free_term_algebra
 structure OpSignature :=
 (operation : Type)
 (arity : operation → Type)
@@ -24,25 +24,47 @@ structure Hom {S : OpSignature} (A : OpAlgebra S) (B : OpAlgebra S) :=
 (op_commute : ∀ (o : S.operation) (args : S.arity o → A.carrier),
 map (A.op o args) = B.op o (λ x, map (args x)))
 
-inductive termtree (S : OpSignature) (X : Type) : Type
-| generator : X → termtree
-| node : ∀ (o : S.operation), (S.arity o → termtree) → termtree
+inductive term {S : OpSignature} (X : Type) : Type
+| gen : X → term
+| node : ∀ (o : S.operation), (S.arity o → term) → term
 
-#check termtree
+#check term
 
 def Free (S : OpSignature) (X : Type) : OpAlgebra S :=
-OpAlgebra.mk (termtree S X) termtree.node
+OpAlgebra.mk 
+  (@term S X) -- carrier 
+  (@term.node S X)   -- operations
 
 #print Free
 
 section free_is_free
+variables (S : OpSignature) (A : OpAlgebra S) 
+variables (X : Type) (h : X → A.carrier) 
 
-variables (S : OpSignature) (X : Type) (A : OpAlgebra S) (h : X → A.carrier)
+def induced_map : (@term S X) → A.carrier
+| (term.gen x) := h x
+| (term.node o args) :=  
+  (A.op o) (λ (i : S.arity o), induced_map (args i))
 
--- That's all I have working so far...
+-- Theorem (Existence): There is a homomorphism from Free S X into every 
+--                      algebra of the given signature.
+theorem induced_hom : Hom (Free S X) A :=
+Hom.mk                      -- construct the homomorphism
+  (induced_map S A X h)          -- the hom map
+  (assume (o: S.operation)       -- proof that the map preserves structure
+    (args : S.arity o → (Free S X).carrier), rfl) 
 
-/- def induced_map : (termtree S X) → A.carrier
-| (generator x) := h x
-| (node o arg) := op A o (λ i, induced_map (arg i))
- -/
+-- Theorem (Uniqueness): The homomorphism in the previous theorem is unique.
+theorem from_free_unique (f g : Hom (Free S X) A) :
+  (∀ (x : X), f.map (term.gen x) = g.map (term.gen x)) → 
+      ∀ (t : @term S X), f.map t = g.map t := 
+      assume h: (∀ (x : X), (f.map (term.gen x) = g.map (term.gen x))),
+      assume (t : @term S X), show (f.map t = g.map t), from sorry
+      --t.rec_on 
+      --(assume x, show f.map (term.gen x) = g.map (term.gen x), from h x)
+      --(assume n, show f.map n = g.map n, sorry)
+      
+  
 
+end free_is_free
+--end free_term_algebra
